save ifc work

Imp.v
@@ -8,3 +8,385 @@ From Coq Require Import List. Import ListNotations.
 From Coq Require Import Strings.String.
 From TL Require Import Maps.
 Set Default Goal Selector "!".
+
+
+
+Module AExp.
+
+Inductive aexp : Type :=
+ | ANum (n : nat)
+ | APlus (a1 a2 : aexp)
+ | AMinus (a1 a2 : aexp)
+ | AMult (a1 a2 : aexp).
+
+Inductive bexp : Type :=
+  | BTrue
+  | BFalse
+  | BEq (a1 a2 : aexp)
+  | BNeq (a1 a2 : aexp)
+  | BLe (a1 a2 : aexp)
+  | BGt (a1 a2 : aexp)
+  | BNot (b : bexp)
+  | BAnd (b1 b2 : bexp).
+
+Fixpoint aeval (a: aexp) : nat :=
+  match a with
+  | ANum n       => n
+  | APlus a1 a2  => (aeval a1) + (aeval a2)
+  | AMinus a1 a2 => (aeval a1) - (aeval a2)
+  | AMult a1 a2  => (aeval a1) * (aeval a2)
+  end.
+
+Example test_aeval1:
+  aeval (APlus (ANum 2) (ANum 3)) = 5.
+Proof. reflexivity. Qed.
+
+Fixpoint beval (b: bexp): bool :=
+  match b with
+  | BTrue        => true
+  | BFalse       => false
+  | BEq a1 a2   => (aeval a1) =? (aeval a2)
+  | BNeq a1 a2  => negb ((aeval a1) =? (aeval a2))
+  | BLe a1 a2   => (aeval a1) <=? (aeval a2)
+  | BGt a1 a2   => negb ((aeval a1) <=? (aeval a2))
+  | BNot b      => negb (beval b)
+  | BAnd b1 b2  => (beval b1) && (beval b2)
+  end.
+
+Fixpoint optimize_0plus (a: aexp): aexp :=
+  match a with
+  | ANum n       => ANum n
+  | APlus (ANum 0) a2 => optimize_0plus a2
+  | APlus a1 a2  => APlus (optimize_0plus a1) (optimize_0plus a2)
+  | AMinus a1 a2 => AMinus (optimize_0plus a1) (optimize_0plus a2)
+  | AMult a1 a2  => AMult (optimize_0plus a1) (optimize_0plus a2)
+  end.
+
+Example test_optimize_0plus:
+  optimize_0plus (APlus (ANum 0) (APlus (ANum 3) (ANum 0)))
+  = APlus (ANum 3) (ANum 0).
+Proof. reflexivity. Qed.
+
+Theorem optimize_0plus_sound:
+  forall a, aeval (optimize_0plus a) = aeval a.
+Proof.
+  intros a. induction a.
+  - (* a = ANum n *) reflexivity.
+  - (* a = APlus a1 a2 *) destruct a1 eqn:Ea1.
+    + (* a1 = ANum n *) destruct n.
+      * (* n = 0 *) simpl. apply IHa2.
+      * (* n <> 0 *) simpl. rewrite IHa2. reflexivity.
+    + (* a1 = APlus a1_1 a1_2 *) simpl. simpl in IHa1. rewrite IHa1. rewrite IHa2. reflexivity.
+    + (* a1 = AMinus a1_1 a1_2 *) simpl. simpl in IHa1. rewrite IHa1.  rewrite IHa2. reflexivity.
+    + (* a1 = AMult a1_1 a1_2 *) simpl. simpl in IHa1. rewrite IHa1. rewrite IHa2. reflexivity.
+  - (* a = AMinus a1 a2 *) simpl. rewrite IHa1. rewrite IHa2. reflexivity.
+  - (* a = AMult a1 a2 *) simpl. rewrite IHa1. rewrite IHa2. reflexivity.
+Qed.
+
+(* ===================== try and ; tactical ======================== *)
+Theorem optimize_0plus_sound':
+  forall a, aeval (optimize_0plus a) = aeval a.
+Proof.
+  intros a. 
+  induction a; 
+    try (simpl; rewrite IHa1; rewrite IHa2; reflexivity).
+  - (* a = ANum n *) reflexivity.
+  - (* a = APlus a1 a2 *) 
+    destruct a1 eqn:Ea1;
+    try (simpl; simpl in IHa1; rewrite IHa1; rewrite IHa2; reflexivity).
+    + (* a1 = ANum n *) destruct n;
+      try (simpl; rewrite IHa2; reflexivity).
+Qed.
+
+Theorem optimize_0plus_sound'':
+  forall a, aeval (optimize_0plus a) = aeval a.
+Proof.
+  intros a. 
+  induction a; 
+    try (simpl; rewrite IHa1; rewrite IHa2; reflexivity);
+    try reflexivity.
+  - (* a = APlus a1 a2 *) 
+    destruct a1 eqn:Ea1;
+    try (simpl; simpl in IHa1; rewrite IHa1; rewrite IHa2; reflexivity).
+    + (* a1 = ANum n *) destruct n;
+      try (simpl; rewrite IHa2; reflexivity).
+Qed.
+
+(* ===================== repeat tactical ======================== *)
+Theorem repeat_loop : forall (m n : nat),
+  m + n = n + m.
+Proof.
+  intros m n.
+  (* rewrite Nat.add_comm. *)
+Admitted.
+
+(* ===================== lia ======================== *)
+Example add_comm__lia: forall m n : nat,
+  m + n = n + m.
+Proof.
+  intros m n. lia.
+Qed.
+
+
+
+End AExp.
+
+
+
+(* ===================== expression with variables ======================== *)
+Definition state := total_map nat.
+Inductive aexp : Type :=
+ | ANum (n : nat)
+ | AId (x : string)
+ | APlus (a1 a2 : aexp)
+ | AMinus (a1 a2 : aexp)
+ | AMult (a1 a2 : aexp).
+
+Inductive bexp : Type :=
+  | BTrue
+  | BFalse
+  | BEq (a1 a2 : aexp)
+  | BNeq (a1 a2 : aexp)
+  | BLe (a1 a2 : aexp)
+  | BGt (a1 a2 : aexp)
+  | BNot (b : bexp)
+  | BAnd (b1 b2 : bexp).
+
+Coercion AId : string >-> aexp.
+Coercion ANum : nat >-> aexp.
+
+Declare Custom Entry com.
+Declare Scope com_scope.
+Declare Custom Entry com_aux.
+
+Notation "<{ e }>" := e (e custom com_aux) : com_scope.
+Notation "e" := e (in custom com_aux at level 0, e custom com) : com_scope.
+
+Notation "( x )" := x (in custom com, x at level 99) : com_scope.
+Notation "x" := x (in custom com at level 0, x constr at level 0) : com_scope.
+Notation "f x .. y" := (.. (f x) .. y)
+                  (in custom com at level 0, only parsing,
+                  f constr at level 0, x constr at level 9,
+                  y constr at level 9) : com_scope.
+Notation "x + y"   := (APlus x y) (in custom com at level 50, left associativity).
+Notation "x - y"   := (AMinus x y) (in custom com at level 50, left associativity).
+Notation "x * y"   := (AMult x y) (in custom com at level 40, left associativity).
+Notation "'true'"  := true (at level 1).
+Notation "'true'"  := BTrue (in custom com at level 0).
+Notation "'false'" := false (at level 1).
+Notation "'false'" := BFalse (in custom com at level 0).
+Notation "x <= y"  := (BLe x y) (in custom com at level 70, no associativity).
+Notation "x > y"   := (BGt x y) (in custom com at level 70, no associativity).
+Notation "x = y"   := (BEq x y) (in custom com at level 70, no associativity).
+Notation "x <> y"  := (BNeq x y) (in custom com at level 70, no associativity).
+Notation "x && y"  := (BAnd x y) (in custom com at level 80, left associativity).
+Notation "'~' b"   := (BNot b) (in custom com at level 75, right associativity).
+
+
+
+Open Scope com_scope.
+
+Fixpoint aeval (st: state) (a: aexp) : nat :=
+  match a with
+  | ANum n       => n
+  | AId x        => st x
+  | APlus a1 a2  => (aeval st a1) + (aeval st a2)
+  | AMinus a1 a2 => (aeval st a1) - (aeval st a2)
+  | AMult a1 a2  => (aeval st a1) * (aeval st a2)
+  end.
+
+Definition W : string := "W".
+Definition X : string := "X".
+Definition Y : string := "Y".
+Definition Z : string := "Z".
+
+Definition empty_st := (_ !-> 0).
+
+Notation "x '!->' v" := (x !-> v ; empty_st) (at level 100).
+
+Example test_aeval1:
+  aeval (X !-> 5) (APlus (ANum 2) (ANum 3)) = 5.
+Proof. reflexivity. Qed.
+
+Example aexp1 :
+    aeval (X !-> 5) <{ 3 + (X * 2) }>
+  = 13.
+Proof. reflexivity. Qed.
+
+Example aexp2 :
+    aeval (t_update (t_update empty_st X 5) Y 4) <{ Z + (X * Y) }>
+  = 20.
+Proof. reflexivity. Qed.  
+
+Fixpoint beval (st: state) (b: bexp): bool :=
+  match b with
+  | BTrue        => true
+  | BFalse       => false
+  | BEq a1 a2   => (aeval st a1) =? (aeval st a2)
+  | BNeq a1 a2  => negb ((aeval st a1) =? (aeval st a2))
+  | BLe a1 a2   => (aeval st a1) <=? (aeval st a2)
+  | BGt a1 a2   => negb ((aeval st a1) <=? (aeval st a2))
+  | BNot b      => negb (beval st b)
+  | BAnd b1 b2  => (beval st b1) && (beval st b2)
+  end.
+
+(* ===================== commands ======================== *)
+Inductive com : Type :=
+  | CSkip
+  | CAsgn (x: string) (a: aexp)
+  | CSeq (c1 c2 : com)
+  | CIf (b: bexp) (c1 c2: com)
+  | CWhile (b: bexp) (c: com).
+
+(* ===================== operational semantics ======================== 
+   define the operational semantics of the Imp language as a function fails:
+
+*)
+
+Fixpoint ceval_fun_no_while (st: state) (c: com) : state :=
+  match c with 
+  | CSkip => st
+  | CAsgn x a => (t_update st x (aeval st a))
+  | CSeq c1 c2 => let st' := ceval_fun_no_while st c1 in
+                  ceval_fun_no_while st' c2
+  | CIf b c1 c2 => if beval st b then ceval_fun_no_while st c1
+                  else ceval_fun_no_while st c2
+  | CWhile b c1 => st (* not allowed *)
+  end.
+
+Notation "'skip'"  :=
+         CSkip (in custom com at level 0) : com_scope.
+Notation "x := y"  :=
+         (CAsgn x y)
+            (in custom com at level 0, x constr at level 0,
+             y at level 85, no associativity) : com_scope.
+Notation "x ; y" :=
+         (CSeq x y)
+           (in custom com at level 90,
+            right associativity) : com_scope.
+Notation "'if' x 'then' y 'else' z 'end'" :=
+         (CIf x y z)
+           (in custom com at level 89, x at level 99,
+            y at level 99, z at level 99) : com_scope.
+Notation "'while' x 'do' y 'end'" :=
+         (CWhile x y)
+           (in custom com at level 89, x at level 99,
+            y at level 99) : com_scope.
+  
+(* The following definition does not work
+    It complains: Cannot guess decreasing argument of fix.
+    because Coq does not accept such a definition that is not guaranteed to terminate.
+ *)
+(* Fixpoint ceval_fun_no_while' (st: state) (c: com) : state :=
+  match c with 
+  | CSkip => st
+  | CAsgn x a => (t_update st x (aeval st a))
+  | CSeq c1 c2 => let st' := ceval_fun_no_while' st c1 in
+                  ceval_fun_no_while' st' c2
+  | CIf b c1 c2 => if beval st b then ceval_fun_no_while' st c1
+                  else ceval_fun_no_while' st c2
+  | CWhile b c1 => if (beval st b) then ceval_fun_no_while' st (CSeq c1 (CWhile b c1))
+                  else st
+  end. *)
+
+  (* A better way is to definition evaluation as a relation *)
+  (** Here is an informal definition of evaluation, presented as inference
+    rules for readability:
+
+                           -----------------                            (E_Skip)
+                           st =[ skip ]=> st
+
+                           aeval st a = n
+                   -------------------------------                      (E_Asgn)
+                   st =[ x := a ]=> (x !-> n ; st)
+
+                           st  =[ c1 ]=> st'
+                           st' =[ c2 ]=> st''
+                         ---------------------                           (E_Seq)
+                         st =[ c1;c2 ]=> st''
+
+                          beval st b = true
+                           st =[ c1 ]=> st'
+                --------------------------------------               (E_IfTrue)
+                st =[ if b then c1 else c2 end ]=> st'
+
+                         beval st b = false
+                           st =[ c2 ]=> st'
+                --------------------------------------              (E_IfFalse)
+                st =[ if b then c1 else c2 end ]=> st'
+
+                         beval st b = false
+                    -----------------------------                 (E_WhileFalse)
+                    st =[ while b do c end ]=> st
+
+                          beval st b = true
+                           st =[ c ]=> st'
+                  st' =[ while b do c end ]=> st''
+                  --------------------------------                 (E_WhileTrue)
+                  st  =[ while b do c end ]=> st''
+*)
+Inductive ceval : com -> state -> state -> Prop :=
+  | E_Skip : forall st, ceval CSkip st st  
+  | E_Asgn : forall st a n x, aeval st a = n ->
+              ceval (CAsgn x a) st (t_update st x n)
+  | E_Seq : forall c1 c2 st st' st'',
+              ceval c1 st st' ->
+              ceval c2 st' st'' ->
+              ceval (CSeq c1 c2) st st''
+  | E_IfTrue : forall st st' b c1 c2,
+                 beval st b = true ->
+                 ceval c1 st st' ->
+                 ceval (CIf b c1 c2) st st'
+  | E_IfFalse : forall st st' b c1 c2,
+                 beval st b = false ->
+                 ceval c2 st st' ->
+                 ceval (CIf b c1 c2) st st'
+  | E_WhileFalse : forall b c st,
+                     beval st b = false ->
+                     ceval (CWhile b c) st st
+  | E_WhileTrue : forall st st' st'' b c,
+                    beval st b = true ->
+                    ceval c st st' ->
+                    ceval (CWhile b c) st' st'' ->
+                    ceval (CWhile b c) st st''.   
+
+Example ceval_example1:
+  ceval <{
+     X := 2;
+     if (X <= 1)
+       then Y := 3
+       else Z := 4
+     end
+  }> empty_st (t_update (t_update empty_st X 2) Z 4).
+Proof.
+  apply E_Seq with (X !-> 2).
+  - apply E_Asgn. reflexivity.
+  - apply E_IfFalse. 
+    + reflexivity.
+    + apply E_Asgn. reflexivity.
+Qed.
+
+Example ceval_example2:
+  ceval <{
+    X := 0;
+    Y := 1;
+    Z := 2
+  }> empty_st (Z !-> 2 ; Y !-> 1 ; X !-> 0).
+Proof.
+  apply E_Seq with (X !-> 0).
+  - apply E_Asgn. reflexivity.
+  - apply E_Seq with (Y !-> 1 ; X !-> 0).
+    + apply E_Asgn. reflexivity.
+    + apply E_Asgn. reflexivity.
+Qed.
+
+Definition plus2 : com :=
+  <{ X := X + 2 }>.
+
+Theorem plus2_spec : forall st n st',
+  st X = n ->
+  ceval plus2 st st' ->
+  st' X = n + 2.
+Proof.
+  intros st n st' HX Hceval.
+  inversion Hceval. subst. simpl. apply t_update_eq. Qed.
