ifc.v
@@ -1,0 +1,377 @@
+Set Warnings "-notation-overridden,-parsing,-deprecated-hint-without-locality".
+From Coq Require Import Bool.
+From Coq Require Import Init.Nat.
+From Coq Require Import Arith.
+From Coq Require Import EqNat. Import Nat.
+From Coq Require Import Lia.
+From Coq Require Import List. Import ListNotations.
+From Coq Require Import Strings.String.
+From TL Require Import Maps.
+Set Default Goal Selector "!".
+
+
+
+(* ===================== expression with variables ======================== *)
+Definition state := total_map nat.
+Inductive aexp : Type :=
+ | ANum (n : nat)
+ | AId (x : string)
+ | APlus (a1 a2 : aexp)
+ | AMinus (a1 a2 : aexp)
+ | AMult (a1 a2 : aexp).
+
+Inductive bexp : Type :=
+  | BTrue
+  | BFalse
+  | BEq (a1 a2 : aexp)
+  | BNeq (a1 a2 : aexp)
+  | BLe (a1 a2 : aexp)
+  | BGt (a1 a2 : aexp)
+  | BNot (b : bexp)
+  | BAnd (b1 b2 : bexp).
+
+Coercion AId : string >-> aexp.
+Coercion ANum : nat >-> aexp.
+
+Declare Custom Entry com.
+Declare Scope com_scope.
+Declare Custom Entry com_aux.
+
+Notation "<{ e }>" := e (e custom com_aux) : com_scope.
+Notation "e" := e (in custom com_aux at level 0, e custom com) : com_scope.
+
+Notation "( x )" := x (in custom com, x at level 99) : com_scope.
+Notation "x" := x (in custom com at level 0, x constr at level 0) : com_scope.
+Notation "f x .. y" := (.. (f x) .. y)
+                  (in custom com at level 0, only parsing,
+                  f constr at level 0, x constr at level 9,
+                  y constr at level 9) : com_scope.
+Notation "x + y"   := (APlus x y) (in custom com at level 50, left associativity).
+Notation "x - y"   := (AMinus x y) (in custom com at level 50, left associativity).
+Notation "x * y"   := (AMult x y) (in custom com at level 40, left associativity).
+Notation "'true'"  := true (at level 1).
+Notation "'true'"  := BTrue (in custom com at level 0).
+Notation "'false'" := false (at level 1).
+Notation "'false'" := BFalse (in custom com at level 0).
+Notation "x <= y"  := (BLe x y) (in custom com at level 70, no associativity).
+Notation "x > y"   := (BGt x y) (in custom com at level 70, no associativity).
+Notation "x = y"   := (BEq x y) (in custom com at level 70, no associativity).
+Notation "x <> y"  := (BNeq x y) (in custom com at level 70, no associativity).
+Notation "x && y"  := (BAnd x y) (in custom com at level 80, left associativity).
+Notation "'~' b"   := (BNot b) (in custom com at level 75, right associativity).
+
+
+
+Open Scope com_scope.
+Definition empty_st := (_ !-> 0).
+
+Notation "x '!->' v" := (x !-> v ; empty_st) (at level 100).
+
+Inductive com : Type :=
+  | CSkip
+  | CAsgn (x: string) (a: aexp)
+  | CSeq (c1 c2 : com)
+  | CIf (b: bexp) (c1 c2: com)
+  | CWhile (b: bexp) (c: com).
+
+Notation "'skip'"  :=
+         CSkip (in custom com at level 0) : com_scope.
+Notation "x := y"  :=
+         (CAsgn x y)
+            (in custom com at level 0, x constr at level 0,
+             y at level 85, no associativity) : com_scope.
+Notation "x ; y" :=
+         (CSeq x y)
+           (in custom com at level 90,
+            right associativity) : com_scope.
+Notation "'if' x 'then' y 'else' z 'end'" :=
+         (CIf x y z)
+           (in custom com at level 89, x at level 99,
+            y at level 99, z at level 99) : com_scope.
+Notation "'while' x 'do' y 'end'" :=
+         (CWhile x y)
+           (in custom com at level 89, x at level 99,
+            y at level 99) : com_scope.
+
+Inductive aval : aexp -> Prop :=
+  | av_num : forall n, aval (ANum n).
+
+Inductive bval : bexp -> Prop :=
+  | bv_true : bval BTrue
+  | bv_false : bval BFalse.
+
+Inductive astep (st: state) : aexp -> aexp -> Prop :=
+  | AS_Id : forall x,
+      astep st (AId x) (ANum (st x))
+  | AS_Plus1 : forall a1 a1' a2,
+      astep st a1 a1' ->
+      astep st (APlus a1 a2) (APlus a1' a2)
+  | AS_Plus2 : forall v1 a2 a2',
+      aval v1 ->
+      astep st a2 a2' ->
+      astep st (APlus v1 a2) (APlus v1 a2')
+  | AS_Plus : forall (n1 n2 : nat),
+      astep st (APlus (ANum n1) (ANum n2)) (ANum (n1 + n2))
+  | AS_Minus1 : forall a1 a1' a2,
+      astep st a1 a1' ->
+      astep st (AMinus a1 a2) (AMinus a1' a2)
+  | AS_Minus2 : forall v1 a2 a2',
+      aval v1 ->
+      astep st a2 a2' ->
+      astep st (AMinus v1 a2) (AMinus v1 a2')
+  | AS_Minus : forall (n1 n2 : nat),
+      astep st (AMinus (ANum n1) (ANum n2)) (ANum (n1 - n2))
+  | AS_Mult1 : forall a1 a1' a2,
+      astep st a1 a1' ->
+      astep st (AMult a1 a2) (AMult a1' a2)
+  | AS_Mult2 : forall v1 a2 a2',
+      aval v1 ->
+      astep st a2 a2' ->
+      astep st (AMult v1 a2) (AMult v1 a2')
+  | AS_Mult : forall (n1 n2 : nat),
+      astep st (AMult (ANum n1) (ANum n2)) (ANum (n1 * n2))
+.
+
+Inductive bstep (st: state) : bexp -> bexp -> Prop :=
+  | BS_Eq1 : forall a1 a1' a2,
+      astep st a1 a1' ->
+      bstep st (BEq a1 a2) (BEq a1' a2)
+  | BS_Eq2 : forall v1 a2 a2',
+      aval v1 ->
+      astep st a2 a2' ->
+      bstep st (BEq v1 a2) (BEq v1 a2')
+  | BS_Eq : forall (n1 n2 : nat),
+      bstep st (BEq (ANum n1) (ANum n2))
+               (if beq_nat n1 n2 then BTrue else BFalse)
+  | BS_Neq1 : forall a1 a1' a2,
+      astep st a1 a1' ->
+      bstep st (BNeq a1 a2) (BNeq a1' a2)
+  | BS_Neq2 : forall v1 a2 a2',
+      aval v1 ->
+      astep st a2 a2' ->
+      bstep st (BNeq v1 a2) (BNeq v1 a2')
+  | BS_Neq : forall (n1 n2 : nat),
+      bstep st (BNeq (ANum n1) (ANum n2))
+               (if beq_nat n1 n2 then BFalse else BTrue)
+  | BS_Le1 : forall a1 a1' a2,
+      astep st a1 a1' ->
+      bstep st (BLe a1 a2) (BLe a1' a2)
+  | BS_Le2 : forall v1 a2 a2',
+      aval v1 ->
+      astep st a2 a2' ->
+      bstep st (BLe v1 a2) (BLe v1 a2')
+  | BS_Le : forall (n1 n2 : nat),
+      bstep st (BLe (ANum n1) (ANum n2))
+               (if n1 <=? n2 then BTrue else BFalse)
+  | BS_Gt1 : forall a1 a1' a2,
+      astep st a1 a1' ->
+      bstep st (BGt a1 a2) (BGt a1' a2)
+  | BS_Gt2 : forall v1 a2 a2',
+      aval v1 ->
+      astep st a2 a2' ->
+      bstep st (BGt v1 a2) (BGt v1 a2')
+  | BS_Gt : forall (n1 n2 : nat),
+      bstep st (BGt (ANum n1) (ANum n2))
+               (if n2 <=? n1 then BTrue else BFalse)
+  | BS_Not1 : forall a1 a1',
+      bstep st a1 a1' ->
+      bstep st (BNot a1) (BNot a1')
+  | BS_NotTrue : 
+      bstep st (BNot BTrue) BFalse
+  | BS_NotFalse : 
+      bstep st (BNot BFalse) BTrue
+  | BS_AndStep : forall b1 b1' b2,
+      bstep st b1 b1' ->
+      bstep st (BAnd b1 b2) (BAnd b1' b2)
+  | BS_AndTrueStep : forall b2 b2',
+      bstep st b2 b2' ->
+      bstep st (BAnd BTrue b2) (BAnd BTrue b2')
+  | BS_AndFalse : forall b2 b2',
+      bstep st b2 b2' ->
+      bstep st (BAnd BFalse b2) BFalse
+  | BS_AndTrueTrue : 
+      bstep st (BAnd BTrue BTrue) BTrue
+  | BS_AndTrueFalse : 
+      bstep st (BAnd BTrue BFalse) BFalse
+.
+
+Inductive cstep : (com * state) -> (com * state) -> Prop :=
+  | CS_AssignStep : forall st x a a',
+      astep st a a' ->
+      cstep (CAsgn x a, st) (CAsgn x a', st)
+  | CS_Assign : forall st x n,
+      cstep (CAsgn x (ANum n), st) (CSkip, (x !-> n ; st))
+  | CS_SeqStep : forall st c1 c1' st' c2,
+      cstep (c1, st) (c1', st') ->
+      cstep (CSeq c1 c2, st) (CSeq c1' c2, st')
+  | CS_SeqFinish : forall st c2,
+      cstep (CSeq CSkip c2, st) (c2, st)
+  | CS_IfStep : forall st b1 b1' c1 c2,
+      bstep st b1 b1' ->
+      cstep (CIf b1 c1 c2, st) (CIf b1' c1 c2, st)
+  | CS_IfTrue : forall st c1 c2,
+      cstep (CIf BTrue c1 c2, st) (c1, st)
+  | CS_IfFalse : forall st c1 c2,
+      cstep (CIf BFalse c1 c2, st) (c2, st)
+  | CS_While : forall st b c,
+      cstep (CWhile b c, st)
+            (CIf b (CSeq c (CWhile b c)) CSkip, st)
+.
+
+Inductive ty : Type :=
+  | L : ty
+  | H : ty.
+
+Definition join (t1 t2 : ty) : ty :=
+  match t1, t2 with
+  | L, L => L
+  | _, _ => H
+  end.
+
+Definition leq_ty (t1 t2 : ty) : Prop :=
+  match t1, t2 with
+  | L, L => True
+  | L, H => True
+  | H, H => True
+  | H, L => False
+  end.
+
+Definition context := total_map ty.
+
+Inductive has_type_aexp : context -> aexp -> ty -> Prop :=
+  | T_ANum : forall Gamma n,
+      has_type_aexp Gamma (ANum n) L
+  | T_AId : forall Gamma x,
+      has_type_aexp Gamma (AId x) (Gamma x)
+  | T_APlus : forall Gamma a1 a2 t1 t2,
+      has_type_aexp Gamma a1 t1 ->
+      has_type_aexp Gamma a2 t2 ->
+      has_type_aexp Gamma (APlus a1 a2) (join t1 t2)
+  | T_AMinus : forall Gamma a1 a2 t1 t2,
+      has_type_aexp Gamma a1 t1 ->
+      has_type_aexp Gamma a2 t2 ->
+      has_type_aexp Gamma (AMinus a1 a2) (join t1 t2)
+  | T_AMult : forall Gamma a1 a2 t1 t2,
+      has_type_aexp Gamma a1 t1 ->
+      has_type_aexp Gamma a2 t2 ->
+      has_type_aexp Gamma (AMult a1 a2) (join t1 t2)
+.
+
+Inductive has_type_bexp : context -> bexp -> ty -> Prop :=
+  | T_BTrue : forall Gamma, has_type_bexp Gamma BTrue L
+  | T_BFalse : forall Gamma, has_type_bexp Gamma BFalse L
+  | T_BEq : forall Gamma a1 a2 t1 t2,
+      has_type_aexp Gamma a1 t1 ->
+      has_type_aexp Gamma a2 t2 ->
+      has_type_bexp Gamma (BEq a1 a2) (join t1 t2)
+  | T_BNeq : forall Gamma a1 a2 t1 t2,
+      has_type_aexp Gamma a1 t1 ->
+      has_type_aexp Gamma a2 t2 ->
+      has_type_bexp Gamma (BNeq a1 a2) (join t1 t2)
+  | T_BLe : forall Gamma a1 a2 t1 t2,
+      has_type_aexp Gamma a1 t1 ->
+      has_type_aexp Gamma a2 t2 ->
+      has_type_bexp Gamma (BLe a1 a2) (join t1 t2)
+  | T_BGt : forall Gamma a1 a2 t1 t2,
+      has_type_aexp Gamma a1 t1 ->
+      has_type_aexp Gamma a2 t2 ->
+      has_type_bexp Gamma (BGt a1 a2) (join t1 t2)
+  | T_BNot : forall Gamma b t,
+      has_type_bexp Gamma b t ->
+      has_type_bexp Gamma (BNot b) t
+  | T_BAnd : forall Gamma b1 b2 t1 t2,
+      has_type_bexp Gamma b1 t1 ->
+      has_type_bexp Gamma b2 t2 ->
+      has_type_bexp Gamma (BAnd b1 b2) (join t1 t2)
+.
+
+Inductive secure_com : context -> ty -> com -> Prop :=
+  | S_Skip : forall Gamma pc,
+      secure_com Gamma pc CSkip
+  | S_Asgn : forall Gamma pc x a t_a,
+      has_type_aexp Gamma a t_a ->
+      leq_ty (join pc t_a) (Gamma x) ->  
+      secure_com Gamma pc (CAsgn x a)
+  | S_Seq : forall Gamma pc c1 c2,
+      secure_com Gamma pc c1 ->
+      secure_com Gamma pc c2 ->
+      secure_com Gamma pc (CSeq c1 c2)
+  | S_If : forall Gamma pc b c1 c2 t_b,
+      has_type_bexp Gamma b t_b ->
+      secure_com Gamma (join pc t_b) c1 ->
+      secure_com Gamma (join pc t_b) c2 ->
+      secure_com Gamma pc (CIf b c1 c2)
+  | S_While : forall Gamma pc b c t_b,
+      has_type_bexp Gamma b t_b ->
+      secure_com Gamma (join pc t_b) c ->
+      secure_com Gamma pc (CWhile b c)
+.
+
+Fixpoint aeval (st: state) (a: aexp) : nat :=
+  match a with
+  | ANum n       => n
+  | AId x        => st x
+  | APlus a1 a2  => (aeval st a1) + (aeval st a2)
+  | AMinus a1 a2 => (aeval st a1) - (aeval st a2)
+  | AMult a1 a2  => (aeval st a1) * (aeval st a2)
+  end.
+
+Fixpoint beval (st: state) (b: bexp): bool :=
+  match b with
+  | BTrue        => true
+  | BFalse       => false
+  | BEq a1 a2   => (aeval st a1) =? (aeval st a2)
+  | BNeq a1 a2  => negb ((aeval st a1) =? (aeval st a2))
+  | BLe a1 a2   => (aeval st a1) <=? (aeval st a2)
+  | BGt a1 a2   => negb ((aeval st a1) <=? (aeval st a2))
+  | BNot b      => negb (beval st b)
+  | BAnd b1 b2  => (beval st b1) && (beval st b2)
+  end.
+
+Inductive ceval : com -> state -> state -> Prop :=
+  | E_Skip : forall st, ceval CSkip st st  
+  | E_Asgn : forall st a n x, aeval st a = n ->
+              ceval (CAsgn x a) st (t_update st x n)
+  | E_Seq : forall c1 c2 st st' st'',
+              ceval c1 st st' ->
+              ceval c2 st' st'' ->
+              ceval (CSeq c1 c2) st st''
+  | E_IfTrue : forall st st' b c1 c2,
+                 beval st b = true ->
+                 ceval c1 st st' ->
+                 ceval (CIf b c1 c2) st st'
+  | E_IfFalse : forall st st' b c1 c2,
+                 beval st b = false ->
+                 ceval c2 st st' ->
+                 ceval (CIf b c1 c2) st st'
+  | E_WhileFalse : forall b c st,
+                     beval st b = false ->
+                     ceval (CWhile b c) st st
+  | E_WhileTrue : forall st st' st'' b c,
+                    beval st b = true ->
+                    ceval c st st' ->
+                    ceval (CWhile b c) st' st'' ->
+                    ceval (CWhile b c) st st''.   
+
+
+Definition low_eq (Gamma : context) (st1 st2 : state) : Prop :=
+  forall x, Gamma x = L -> st1 x = st2 x.
+
+Theorem noninterference_soundness :
+  forall Gamma pc c st1 st2 st1' st2',
+    (* if the syntatic judgment \Gamma\vdash_{pc} c secure is derivable *)
+    secure_com Gamma pc c ->
+    (* then non-interference holds, i.e. *)
+    low_eq Gamma st1 st2 ->
+    ceval c st1 st1' ->
+    ceval c st2 st2' ->
+    low_eq Gamma st1' st2'.
+  Proof.
+  intros Gamma pc c st1 st2 st1' st2' Hsec Hloweq He1 He2.
+  induction Hsec.
+  - (* S_Skip *) inversion He1. inversion He2. subst. auto.
+  - (* S_Asgn *) inversion He1. inversion He2. 
+    intros xx HxL.
+  - (* S_Seq *) inversion He1. inversion He2. subst. auto.
+  - (* S_If *) inversion He1. inversion He2. subst. auto.
+  - (* S_While *) inversion He1. inversion He2. subst. auto.
